need better trace, but otherwise looks promising

theories/Logic/inverse_neg_omega.v
@@ -15,7 +15,7 @@ From Systems Require Import proof_trees.
 From Systems Require Import substitute.
 Require Import Lia.
 Require Import Coq.Logic.Eqdep_dec.
-
+Require Import Datatypes.
 
 
 Definition neg_w_rule_sub_formula
@@ -136,7 +136,7 @@ match P , S with
       A
       (neg_w_rule_sub_formula D E n t S_D)
       k d alpha (fun p => 
-      (neg_w_rule_sub_ptree_fit (g p) E n t (S_D)))
+      (neg_w_rule_sub_ptree_fit (g p) E n t (lor_ind (non_target A) (S_D))))
 
 | cut_ca C0 A d1 d2 alpha1 alpha2 P1 P2, _ =>
     cut_ca
@@ -172,6 +172,7 @@ match subst_ind_fit (ptree_formula P) S with
 | true => neg_w_rule_sub_ptree_fit P E n t S
 end.
 
+(**)
 Fixpoint neg_w_rule_trace
   (P : ptree) (S : subst_ind) : subst_ind :=
 match P , S with
@@ -183,6 +184,41 @@ match P , S with
     | true => lor_ind S_A (non_target D)
     | false => S
     end
+
+| _,_ => S
+end.
+
+Fixpoint neg_w_rule_trace_2
+  (P : ptree) (S : subst_ind) : subst_ind :=
+match P , S with
+| deg_up d P', _ => neg_w_rule_trace_2 P' S
+
+| ord_up alpha P', _ => neg_w_rule_trace_2 P' S
+
+| exchange_ab A B d alpha P', lor_ind S_A S_B => (neg_w_rule_trace_2 P' (lor_ind S_B S_A))
+
+| exchange_cab C A B d alpha P', lor_ind (lor_ind S_C S_B) S_A  => (neg_w_rule_trace_2 P' (lor_ind (lor_ind S_C S_A) S_B))
+
+| exchange_abd A B D d alpha P', lor_ind (lor_ind S_B S_A) S_D => (neg_w_rule_trace_2 P' (lor_ind (lor_ind S_A S_B) S_D))
+
+| exchange_cabd C0 A B D d alpha P', lor_ind (lor_ind (lor_ind S_C S_B) S_A) S_D => (neg_w_rule_trace_2 P' (lor_ind (lor_ind (lor_ind S_C S_A) S_B) S_D))
+
+| contraction_a A d alpha P', _ => (neg_w_rule_trace_2 P' (lor_ind S S))
+
+| contraction_ad A D d alpha P', lor_ind S_A S_D => (neg_w_rule_trace_2 P' (lor_ind (lor_ind S_A S_A) S_D))
+
+| weakening_ad A D d alpha P', lor_ind S_A S_D => (lor_ind (target A) (neg_w_rule_trace_2 P' S_D))
+
+| demorgan_abd A B D d1 d2 alpha1 alpha2 P1 P2, lor_ind S_AB S_D => (lor_ind (0) (neg_w_rule_trace_2 P1 (lor_ind (0) S_D)))
+
+| negation_ad A D d alpha P', lor_ind S_A S_D => lor_ind (0) (neg_w_rule_trace_2 P' (lor_ind (non_target A) S_D))
+
+| quantification_ad A D k r d alpha P', lor_ind S_A S_D => match (subst_ind_fit D S_D) with
+    | true => lor_ind S_A (non_target D)
+    | false => S
+    end
+
+| w_rule_ad A D k d alpha g, lor_ind S_A S_D => (lor_ind (0) (neg_w_rule_trace_2 (g 0) S_D))
 
 | _,_ => S
 end.
@@ -209,7 +245,7 @@ Proof.
 intros. rewrite neg_w_rule_ptree_formula_aux'.
 - unfold neg_w_rule_sub_formula. rewrite sub_fit_false. auto. apply H.
 - apply H.
-Qed.
+Defined.
 
 Lemma neg_w_rule_ptree_formula_true :
   forall (P : ptree) (E : formula) (n : nat) (t : term) (S : subst_ind),
@@ -221,43 +257,75 @@ Lemma neg_w_rule_trace_fits : forall P S, subst_ind_fit (ptree_formula P) S = tr
 Proof.
 intros P. induction P; auto.
 intros. simpl. destruct S; inversion H. destruct S1; inversion H; rewrite H2; rewrite non_target_fit; auto.
-Qed.
+Defined.
 
 Lemma neg_w_rule_trace_fits_not : forall P S, subst_ind_fit (ptree_formula P) S = false -> subst_ind_fit (ptree_formula P) (neg_w_rule_trace P S) = false.
 Proof.
 intros P. induction P; auto.
 intros. simpl. destruct S; auto. destruct S1; inversion H; try rewrite H1; try rewrite H1; auto. case (subst_ind_fit f0 S2); auto.
-Qed.
+Defined.
 
-Lemma neg_w_rule_ptree_formula' : forall (P : ptree) (E : formula) (n : nat),
-  valid P ->
-  forall (S : subst_ind),
-    subst_ind_fit (ptree_formula P) S = true ->
-    {t : term & closed_t t = true /\ ptree_formula (neg_w_rule_sub_ptree P E n t (neg_w_rule_trace P S)) = neg_w_rule_sub_formula (ptree_formula P) E n t (neg_w_rule_trace P S)}.
+Definition neg_w_rule_term (P : ptree) (E : formula) (n : nat) (H : valid P) : forall (S : subst_ind), subst_ind_fit (ptree_formula P) S = true -> term.
+induction P; intros.
+- destruct H. simpl in H0. apply (IHP v S). auto.
+- destruct H as [[X1 X2] X3]. simpl in H0. apply (IHP X2 S). auto.
+- intros. exact zero.
+- destruct H as [[[X1 X2] X3] X4]; destruct S; inversion H0; apply (IHP X2 (lor_ind S2 S1)); auto. rewrite X1. simpl. apply and_bool_symm; auto.
+- destruct H as [[[X1 X2] X3] X4]; destruct S; inversion H0; destruct S1; inversion H0; apply (IHP X2 (lor_ind (lor_ind S1_1 S2) S1_2)); auto. rewrite X1. simpl. apply and_bool_prop in H1; destruct H1. rewrite H1. apply and_bool_prop in H; destruct H. rewrite H. auto.
+- destruct H as [[[X1 X2] X3] X4]; destruct S; inversion H0; destruct S1; inversion H0; apply (IHP X2 (lor_ind (lor_ind S1_2 S1_1) S2)); auto. rewrite X1. simpl. apply and_bool_prop in H1; destruct H1. rewrite H1. apply and_bool_prop in H; destruct H. rewrite H. rewrite H3. auto.
+- destruct H as [[[X1 X2] X3] X4]; destruct S; inversion H0; destruct S1; inversion H0; destruct S1_1; inversion H0; apply (IHP X2 (lor_ind (lor_ind (lor_ind S1_1_1 S1_2) S1_1_2) S2)); auto. rewrite X1. simpl. apply and_bool_prop in H1; destruct H1. rewrite H1. apply and_bool_prop in H; destruct H. apply and_bool_prop in H; destruct H. rewrite H. rewrite H4. rewrite H5. auto.
+- destruct H as [[[X1 X2] X3] X4]; apply (IHP X2 (lor_ind S S)); auto. rewrite X1. simpl. simpl in H0. rewrite H0. auto.
+- destruct H as [[[X1 X2] X3] X4]; destruct S; inversion H0. apply (IHP X2 (lor_ind (lor_ind S1 S1) S2)); auto. rewrite X1. simpl. apply and_bool_prop in H1. destruct H1. rewrite H1. rewrite H. auto.
+- destruct H as [[[[X1 X2] X3] X4] X5]; destruct S; inversion H0; apply (IHP X3 S2); auto. rewrite X1. apply and_bool_prop in H1. destruct H1. auto.
+- destruct H as [[[[[[X1 X2] X3] X4] X5] X6] X7]; apply (IHP2 X3 S); auto. rewrite X2. destruct S; inversion H0; auto.
+- destruct H as [[[[[[X1 X2] X3] X4] X5] X6] X7]; apply (IHP2 X3 S); auto. rewrite X2. destruct S; inversion H0; auto.
+- destruct H as [[[X1 X2] X3] X4]; destruct S; inversion H0; auto. apply (IHP X2 (non_target f)); auto. rewrite X1. apply non_target_fit. apply (IHP X2 (target f)); auto. rewrite X1. apply target_fit.
+- destruct H as [[[X1 X2] X3] X4]; destruct S; inversion H0; auto; destruct S1;inversion H0. apply (IHP X2 (lor_ind (non_target f) S2)); auto. rewrite X1. simpl. rewrite non_target_fit. auto. apply (IHP X2 (lor_ind (target f) S2)); auto. rewrite X1. simpl. rewrite target_fit. auto.
+- case (eq_nat n0 n). case (eq_f f E). destruct S; inversion H0. destruct H as [[[[X1 X2] X3] X4] X5]; apply (IHP X3 (0)); auto. rewrite X1. auto. exact t. destruct H as [[[[X1 X2] X3] X4] X5]; apply (IHP X3 S); auto. rewrite X1. simpl in H0. simpl. rewrite H0. auto. destruct H as [[[[X1 X2] X3] X4] X5]; apply (IHP X3 S); auto. rewrite X1. simpl in H0. simpl. rewrite H0. auto.
+- case (eq_nat n0 n). case (eq_f f E). destruct S; inversion H0. destruct S1; inversion H0. destruct H as [[[[X1 X2] X3] X4] X5]; apply (IHP X3 (lor_ind (0) S2)); auto. rewrite X1. auto. exact t. destruct H as [[[[X1 X2] X3] X4] X5]; apply (IHP X3 S); auto. rewrite X1. simpl in H0. simpl. rewrite H0. auto. destruct H as [[[[X1 X2] X3] X4] X5]; apply (IHP X3 S); auto. rewrite X1. simpl in H0. simpl. rewrite H0. auto.
+- destruct (H 0) as [[[X1 X2] X3] X4]. fold valid in X2. destruct S; inversion H0. apply (X 0 X2 (non_target f)). rewrite X1. rewrite (non_target_term_sub f n0 zero). apply non_target_fit. apply (X 0 X2 (target f)). rewrite X1. rewrite (target_term_sub f n0 zero). apply target_fit.
+- destruct (H 0) as [[[X1 X2] X3] X4]. fold valid in X2. destruct S; inversion H0. destruct S1; inversion H0. apply (X 0 X2 (lor_ind (non_target f) S2)). rewrite X1. rewrite (non_target_term_sub f n0 zero). simpl. rewrite non_target_fit. auto. apply (X 0 X2 (lor_ind (target f) S2)). rewrite X1. simpl. rewrite (target_term_sub f n0 zero). rewrite target_fit. auto.
+- destruct H as [[[[[[[X1 X2] X3] X4] X5] X6] X7] X8]; apply (IHP1 X2 (lor_ind S (non_target f0))); auto. rewrite X1. simpl. simpl in H0. rewrite H0. apply non_target_fit.
+- destruct H as [[[[[[[X1 X2] X3] X4] X5] X6] X7] X8]; apply (IHP2 X4 (lor_ind (0) S)); auto. rewrite X3. simpl. simpl in H0. apply H0.
+- destruct H as [[[[[[[X1 X2] X3] X4] X5] X6] X7] X8]; destruct S; inversion H0. apply (IHP2 X4 (lor_ind (0) S2)); auto. rewrite X3. simpl. apply and_bool_prop in H1. destruct H1. auto.
+Defined.
+
+Lemma term_helper1 : forall f n0 t n1 o P Hs X1 X2 X3 X4 X5, eq_term (neg_w_rule_term (quantification_a f n0 t n1 o P) f n0 (X1, X2, X3, X4, X5) (1) Hs) t = true.
+Proof.
+fold valid. intros. simpl. rewrite eq_nat_refl. rewrite eq_f_refl. destruct Hs. simpl. apply eq_term_refl.
+Defined.
+
+Lemma term_helper2 : forall f f0 n0 t n1 o P S Hs X1 X2 X3 X4 X5, eq_term (neg_w_rule_term (quantification_ad f f0 n0 t n1 o P) f n0 (X1, X2, X3, X4, X5) (lor_ind (1) S) Hs) t = true.
+Proof.
+fold valid. intros. simpl. assert (negb false = true). auto. rewrite eq_nat_refl. rewrite eq_f_refl. destruct Hs. simpl. rewrite eq_term_refl. simpl in H. auto.
+Defined.
+
+Lemma neg_w_rule_ptree_formula : forall (P : ptree) (E : formula) (n : nat) (H : valid P) (S : subst_ind) (Hs: subst_ind_fit (ptree_formula P) S = true),
+    ptree_formula (neg_w_rule_sub_ptree P E n (neg_w_rule_term P E n H S Hs) (neg_w_rule_trace P S)) = neg_w_rule_sub_formula (ptree_formula P) E n (neg_w_rule_term P E n H S Hs) (neg_w_rule_trace P S).
 Proof.
 intros P E n.
 induction P; try intros H S Hs; unfold neg_w_rule_trace; fold neg_w_rule_trace.
 
-- unfold neg_w_rule_sub_ptree. simpl. rewrite neg_w_rule_trace_fits; auto. destruct H as [H1 H2]. simpl in Hs. simpl. destruct (IHP H2 S Hs) as [r [Hc Hr]]. exists r; auto. rewrite neg_w_rule_ptree_formula_true; auto. rewrite neg_w_rule_trace_fits; auto.
+- unfold neg_w_rule_sub_ptree. simpl. rewrite neg_w_rule_trace_fits; auto. destruct H as [H1 H2]. simpl in Hs. simpl. destruct (IHP H2 S Hs). rewrite neg_w_rule_ptree_formula_true; auto. rewrite neg_w_rule_trace_fits; auto.
 
-- unfold neg_w_rule_sub_ptree. simpl. rewrite neg_w_rule_trace_fits; auto. destruct H as [[H1 H2] H3]. simpl in Hs. simpl. destruct (IHP H2 S Hs) as [r [Hc Hr]]. exists r; auto. rewrite neg_w_rule_ptree_formula_true; auto. rewrite neg_w_rule_trace_fits; auto.
+- unfold neg_w_rule_sub_ptree. simpl. rewrite neg_w_rule_trace_fits; auto. destruct H as [[H1 H2] H3]. simpl in Hs. simpl. destruct (IHP H2 S Hs). rewrite neg_w_rule_ptree_formula_true; auto. rewrite neg_w_rule_trace_fits; auto.
 
-- exists zero; auto. simpl. inversion H. destruct (axiom_atomic _ H); destruct H0; rewrite H0;
+- simpl. inversion H. destruct (axiom_atomic _ H); destruct H0; rewrite H0;
   unfold neg_w_rule_sub_formula; simpl; destruct S; auto.
 
-- exists zero; auto. simpl. destruct S; inversion Hs; rewrite neg_w_rule_simp; simpl; auto; unfold neg_w_rule_sub_formula.
+- simpl. destruct S; inversion Hs; rewrite neg_w_rule_simp; simpl; auto; unfold neg_w_rule_sub_formula.
   rewrite formula_sub_ind_lor; auto.
 
-- exists zero; auto. simpl. destruct S; try destruct S1; inversion Hs; rewrite neg_w_rule_simp; simpl; auto; unfold neg_w_rule_sub_formula.
+- simpl. destruct S; try destruct S1; inversion Hs; rewrite neg_w_rule_simp; simpl; auto; unfold neg_w_rule_sub_formula.
   rewrite formula_sub_ind_lor, formula_sub_ind_lor; auto.
   apply (and_bool_prop _ _ H1).
 
-- exists zero; auto. simpl. destruct S; try destruct S1; inversion Hs; rewrite neg_w_rule_simp; simpl; auto;
+- simpl. destruct S; try destruct S1; inversion Hs; rewrite neg_w_rule_simp; simpl; auto;
   unfold neg_w_rule_sub_formula.
   rewrite formula_sub_ind_lor, formula_sub_ind_lor; auto.
   apply (and_bool_prop _ _ H1).
 
-- exists zero; auto. simpl. destruct S; simpl.
+- simpl. destruct S; simpl.
   + unfold neg_w_rule_sub_formula. auto.
   + unfold neg_w_rule_sub_formula. auto.
   + destruct S1; try destruct S1_1; inversion Hs.
@@ -265,24 +333,24 @@ induction P; try intros H S Hs; unfold neg_w_rule_trace; fold neg_w_rule_trace.
     destruct (and_bool_prop _ _ H1). destruct (and_bool_prop _ _ H0).
     repeat rewrite formula_sub_ind_lor; auto.
 
-- exists zero; auto. simpl. inversion Hs. rewrite neg_w_rule_simp; simpl; auto.
+- simpl. inversion Hs. rewrite neg_w_rule_simp; simpl; auto.
 
-- exists zero; auto. simpl. destruct S; inversion Hs.
+- simpl. destruct S; inversion Hs.
   rewrite neg_w_rule_simp; simpl; auto. unfold neg_w_rule_sub_formula.
   rewrite formula_sub_ind_lor. auto. apply H1.
 
-- exists zero; auto. simpl. destruct S; auto. inversion Hs. rewrite neg_w_rule_simp; simpl; auto.
+- simpl. destruct S; auto. inversion Hs. rewrite neg_w_rule_simp; simpl; auto.
   unfold neg_w_rule_sub_formula. rewrite formula_sub_ind_lor. auto. apply H1.
 
-- exists zero; auto. simpl. destruct S; auto.
+- simpl. destruct S; auto.
 
-- exists zero; auto. simpl. destruct S.
+- simpl. destruct S.
   + inversion Hs.
   + inversion Hs.
   + destruct S1; inversion Hs; rewrite neg_w_rule_simp; simpl; auto; unfold neg_w_rule_sub_formula;
     rewrite formula_sub_ind_lor; auto; apply H1.
 
-- exists zero; auto. simpl. destruct (eq_f f E) eqn:Heq; destruct S.
+- simpl. destruct (eq_f f E) eqn:Heq; destruct S.
   + simpl. unfold neg_w_rule_sub_formula. rewrite formula_sub_ind_0. auto.
   + unfold neg_w_rule_sub_formula. simpl. inversion H as [[[H1 H2] H3] H4]. auto.
   + inversion Hs.
@@ -290,85 +358,83 @@ induction P; try intros H S Hs; unfold neg_w_rule_trace; fold neg_w_rule_trace.
   + unfold neg_w_rule_sub_formula. simpl. auto.
   + inversion Hs.
 
-- exists zero; auto. simpl. destruct (eq_f f E) eqn:Heq; destruct S.
+- simpl in Hs. destruct (eq_f f E) eqn:Heq; destruct S.
   + inversion Hs.
   + inversion Hs.
   + destruct S1.
-    * apply (subst_ind_fit_lor) in Hs. destruct (and_bool_prop _ _ Hs).
-    rewrite neg_w_rule_simp; simpl; auto. unfold neg_w_rule_sub_formula.
-      rewrite formula_sub_ind_lor, formula_sub_ind_0. auto. apply Hs.
-    * inversion Hs. rewrite neg_w_rule_simp; simpl; auto. inversion H as [[[H2 H3] H4] H5].
-      unfold neg_w_rule_sub_formula. simpl. rewrite H1. rewrite sub_fit_true; auto.
-    * simpl. inversion Hs.
-  + inversion Hs.
-  + inversion Hs.
-  + destruct S1.
-    * apply (subst_ind_fit_lor) in Hs. destruct (and_bool_prop _ _ Hs).
+    * destruct H as [[[X1 X2] X3] X4]. simpl. 
       rewrite neg_w_rule_simp; simpl; auto. unfold neg_w_rule_sub_formula.
+      rewrite formula_sub_ind_lor, formula_sub_ind_0. auto. apply Hs.
+    * inversion Hs. rewrite neg_w_rule_simp; simpl; auto. destruct H as [[[H2 H3] H4] H5].
+      unfold neg_w_rule_sub_formula. simpl. rewrite H1 at 1. rewrite sub_fit_true; auto.
+    * inversion Hs.
+  + inversion Hs.
+  + inversion Hs.
+  + destruct S1.
+    * rewrite neg_w_rule_simp; simpl; auto. unfold neg_w_rule_sub_formula.
       rewrite formula_sub_ind_lor, formula_sub_ind_0. auto. apply Hs.
     * inversion Hs. rewrite neg_w_rule_simp; simpl; auto. unfold neg_w_rule_sub_formula.
       rewrite formula_sub_ind_lor; auto.
     * simpl. inversion Hs.
 
-- simpl. destruct H as [[[[X1 X2] X3] X4] X5]. case (eq_f f E) eqn:Y; case (eq_nat n0 n) eqn:Y1.
-  + exists t; auto. apply f_eq_decid in Y. destruct Y. apply nat_eq_decid in Y1. destruct Y1. destruct S.
-    * rewrite neg_w_rule_simp; auto. unfold neg_w_rule_sub_formula. unfold formula_sub_ind. unfold subst_ind_fit. unfold formula_sub_ind_fit. rewrite eq_f_refl. unfold neg_w_rule_sub_ptree_fit. rewrite eq_f_refl. rewrite eq_nat_refl. rewrite eq_term_refl. simpl. auto.
-    * rewrite neg_w_rule_simp; auto. unfold neg_w_rule_sub_formula. unfold formula_sub_ind. unfold subst_ind_fit. unfold formula_sub_ind_fit. rewrite eq_f_refl. unfold neg_w_rule_sub_ptree_fit. rewrite eq_f_refl. rewrite eq_nat_refl. rewrite eq_term_refl. simpl. auto.
+- destruct H as [[[[X1 X2] X3] X4] X5]. case (eq_f f E) eqn:Y; case (eq_nat n0 n) eqn:Y1.
+  + apply f_eq_decid in Y. destruct Y. apply nat_eq_decid in Y1. destruct Y1. destruct S.
+    * rewrite neg_w_rule_simp; auto. unfold neg_w_rule_sub_formula. unfold ptree_formula. fold ptree_formula. unfold formula_sub_ind. unfold formula_sub_ind_fit. rewrite eq_f_refl. unfold ptree_formula in Hs. rewrite Hs at 1.
+      unfold neg_w_rule_sub_ptree_fit. rewrite eq_f_refl. rewrite eq_nat_refl. case (eq_term (neg_w_rule_term (quantification_a f n0 t n1 o P) f n0 (X1, X2, X3, X4, X5) (0) Hs) t); auto.
+    * rewrite neg_w_rule_simp; auto. unfold neg_w_rule_sub_formula. unfold ptree_formula. fold ptree_formula. unfold formula_sub_ind. unfold subst_ind_fit. unfold formula_sub_ind_fit. rewrite eq_f_refl. unfold neg_w_rule_sub_ptree_fit. rewrite eq_f_refl. rewrite eq_nat_refl.
+      rewrite term_helper1. unfold ptree_formula. fold ptree_formula. pose proof (term_helper1 f n0 t n1 o P Hs X1 X2 X3 X4 X5). apply term_beq_eq in H. rewrite X1 at 1. rewrite <- H at 1. auto.
     * inversion Hs.
-  + exists zero; auto. destruct S; rewrite neg_w_rule_simp; simpl; auto; unfold neg_w_rule_sub_formula; simpl; try rewrite Y; try rewrite Y1; auto.
-  + exists zero; auto. destruct S; rewrite neg_w_rule_simp; simpl; auto; unfold neg_w_rule_sub_formula; simpl; try rewrite Y; try rewrite Y1;  auto.
-  + exists zero; auto. destruct S; rewrite neg_w_rule_simp; simpl; auto; unfold neg_w_rule_sub_formula; simpl; try rewrite Y; try rewrite Y1;  auto.
+  + destruct S; rewrite neg_w_rule_simp; simpl; auto; unfold neg_w_rule_sub_formula; simpl; try rewrite Y; try rewrite Y1; auto.
+  + destruct S; rewrite neg_w_rule_simp; simpl; auto; unfold neg_w_rule_sub_formula; simpl; try rewrite Y; try rewrite Y1;  auto.
+  + destruct S; rewrite neg_w_rule_simp; simpl; auto; unfold neg_w_rule_sub_formula; simpl; try rewrite Y; try rewrite Y1;  auto.
 
-- simpl. destruct H as [[[[X1 X2] X3] X4] X5]. case (eq_f f E) eqn:Y; case (eq_nat n0 n) eqn:Y1.
-  + exists t; split; auto. apply f_eq_decid in Y. destruct Y. apply nat_eq_decid in Y1. destruct Y1. destruct S.
+- destruct H as [[[[X1 X2] X3] X4] X5]. case (eq_f f E) eqn:Y; case (eq_nat n0 n) eqn:Y1.
+  + apply f_eq_decid in Y. destruct Y. apply nat_eq_decid in Y1. destruct Y1. destruct S.
     * rewrite neg_w_rule_simp; auto.
     * rewrite neg_w_rule_simp; auto. 
-    * assert (subst_ind_fit f0 S2 = true) as Z. destruct S1; inversion Hs; auto. rewrite Z. rewrite neg_w_rule_simp; auto. unfold neg_w_rule_sub_formula. rewrite formula_sub_ind_lor; auto. destruct S1; inversion Hs.
-      --  repeat rewrite sub_fit_true; auto; try rewrite non_target_fit; auto. simpl. rewrite eq_f_refl. rewrite eq_nat_refl. rewrite eq_term_refl. simpl. unfold neg_w_rule_sub_formula. rewrite sub_fit_true; auto; rewrite non_target_fit. auto.
-      --  repeat rewrite sub_fit_true; auto; try rewrite non_target_fit; auto. simpl. rewrite eq_f_refl. rewrite eq_nat_refl. rewrite eq_term_refl. simpl. rewrite X1. rewrite non_target_sub'. auto.
+    * assert (subst_ind_fit f0 S2 = true) as Z. destruct S1; inversion Hs; auto. rewrite Z. rewrite neg_w_rule_simp; auto. unfold neg_w_rule_sub_formula. unfold ptree_formula. fold ptree_formula. rewrite formula_sub_ind_lor; auto. destruct S1; inversion Hs.
+      --  repeat rewrite sub_fit_true; auto; try rewrite non_target_fit; auto. unfold formula_sub_ind_fit. fold formula_sub_ind_fit. rewrite eq_f_refl. 
+          unfold neg_w_rule_sub_ptree_fit. fold neg_w_rule_sub_ptree_fit. rewrite eq_f_refl. rewrite eq_nat_refl.
+          case (eq_term (neg_w_rule_term (quantification_ad f f0 n0 t n1 o P) f n0 (X1, X2, X3, X4, X5) (lor_ind (0) S2) Hs) t); auto; unfold ptree_formula; unfold neg_w_rule_sub_formula; rewrite sub_fit_true; auto; apply non_target_fit.
+      --  repeat rewrite sub_fit_true; auto; try rewrite non_target_fit; auto. unfold formula_sub_ind_fit. fold formula_sub_ind_fit. rewrite eq_f_refl. 
+          unfold neg_w_rule_sub_ptree_fit. fold neg_w_rule_sub_ptree_fit. rewrite eq_f_refl. rewrite eq_nat_refl.
+          rewrite term_helper2. unfold ptree_formula. fold ptree_formula. pose proof (term_helper2 f f0 n0 t n1 o P S2 Hs X1 X2 X3 X4 X5). apply term_beq_eq in H. rewrite X1 at 1. rewrite <- H at 1. rewrite non_target_sub'. auto.
       --  rewrite non_target_fit. destruct S1; inversion Hs; auto.
       --  simpl. rewrite non_target_fit. destruct S1; inversion Hs; try rewrite H0; auto.
-  + exists zero; auto. destruct S.
+  + destruct S.
     * simpl. unfold neg_w_rule_sub_formula. simpl. auto.
     * simpl. unfold neg_w_rule_sub_formula. simpl. auto.
     * assert (subst_ind_fit f0 S2 = true) as Z. destruct S1; inversion Hs; auto. rewrite Z. destruct S1; inversion Hs; rewrite neg_w_rule_simp; simpl; auto; try rewrite non_target_fit; auto; unfold neg_w_rule_sub_formula; rewrite Y,Y1; simpl; rewrite Y,Y1; simpl; rewrite non_target_fit; try rewrite H0; try rewrite sub_fit_true; try rewrite non_target_fit; auto.
-  + exists zero; auto. destruct S.
+  + destruct S.
     * simpl. unfold neg_w_rule_sub_formula. simpl. auto.
     * simpl. unfold neg_w_rule_sub_formula. simpl. auto.
-    * destruct S1; inversion Hs; rewrite neg_w_rule_simp; simpl; auto; try rewrite non_target_fit; auto; unfold neg_w_rule_sub_formula;  try rewrite Y,Y1; simpl; try rewrite non_target_fit; auto; try rewrite Y,Y1; simpl; try rewrite H0; try rewrite sub_fit_true; try rewrite non_target_fit; auto.
-  + exists zero; auto. destruct S.
+    * inversion Hs. apply and_bool_prop in H0. destruct H0. rewrite H0.
+      destruct S1; inversion Hs; rewrite neg_w_rule_simp; simpl; auto; try rewrite non_target_fit; auto; unfold neg_w_rule_sub_formula;  try rewrite Y,Y1; simpl; try rewrite non_target_fit; auto; try rewrite Y,Y1; simpl; try rewrite H0; try rewrite sub_fit_true; try rewrite non_target_fit; auto.
+  + destruct S.
     * simpl. unfold neg_w_rule_sub_formula. simpl. auto.
     * simpl. unfold neg_w_rule_sub_formula. simpl. auto.
     * assert (subst_ind_fit f0 S2 = true) as Z. destruct S1; inversion Hs; auto. rewrite Z. destruct S1; inversion Hs; rewrite neg_w_rule_simp; simpl; auto; try rewrite non_target_fit; auto; unfold neg_w_rule_sub_formula; simpl; try rewrite non_target_fit; auto; try rewrite Y,Y1; simpl; try rewrite Y,Y1; simpl; try rewrite H0; rewrite sub_fit_true; try rewrite non_target_fit; auto.
 
-- exists zero; auto. intros. simpl. destruct S; auto.
+- intros. simpl. destruct S; auto.
 
-- exists zero; auto. intros. simpl. destruct S; auto. destruct S1; auto. 
-  + destruct (subst_ind_fit f0 S2) eqn:HS2; rewrite neg_w_rule_simp; simpl; auto.
-    * unfold neg_w_rule_sub_formula. simpl. rewrite HS2. rewrite sub_fit_true; auto.
-    * unfold neg_w_rule_sub_formula. simpl. rewrite HS2. rewrite sub_fit_false; auto.
-  + destruct (subst_ind_fit f0 S2) eqn:HS2; rewrite neg_w_rule_simp; simpl; auto.
-    * unfold neg_w_rule_sub_formula. simpl. rewrite HS2. rewrite sub_fit_true; auto.
-    * unfold neg_w_rule_sub_formula. simpl. rewrite HS2. rewrite sub_fit_false; auto.
+- intros. destruct S; auto. destruct S1; auto. 
+  + destruct (subst_ind_fit f0 S2) eqn:HS2; rewrite neg_w_rule_simp; auto.
+    * unfold neg_w_rule_sub_formula. unfold ptree_formula. fold ptree_formula. unfold formula_sub_ind.  unfold subst_ind_fit. fold subst_ind_fit. rewrite HS2. unfold "&&".  unfold neg_w_rule_sub_ptree_fit. fold neg_w_rule_sub_ptree_fit.
+      unfold formula_sub_ind_fit. fold formula_sub_ind_fit. unfold eq_f. unfold ptree_formula. rewrite <- sub_fit_true; auto.
+    * unfold neg_w_rule_sub_formula. unfold ptree_formula. fold ptree_formula. unfold formula_sub_ind.  unfold subst_ind_fit. fold subst_ind_fit. rewrite HS2. unfold "&&".  unfold neg_w_rule_sub_ptree_fit. fold neg_w_rule_sub_ptree_fit.
+      unfold formula_sub_ind_fit. fold formula_sub_ind_fit. unfold eq_f. unfold ptree_formula. unfold neg_w_rule_sub_formula. rewrite sub_fit_false; auto.
+  + destruct (subst_ind_fit f0 S2) eqn:HS2; rewrite neg_w_rule_simp; auto.
+    * unfold neg_w_rule_sub_formula. unfold ptree_formula. fold ptree_formula. unfold formula_sub_ind.  unfold subst_ind_fit. fold subst_ind_fit. rewrite HS2. unfold "&&".  unfold neg_w_rule_sub_ptree_fit. fold neg_w_rule_sub_ptree_fit.
+      unfold formula_sub_ind_fit. fold formula_sub_ind_fit. unfold eq_f. unfold ptree_formula. rewrite <- sub_fit_true; auto.
+    * unfold neg_w_rule_sub_formula. unfold ptree_formula. fold ptree_formula. unfold formula_sub_ind.  unfold subst_ind_fit. fold subst_ind_fit. rewrite HS2. unfold "&&".  unfold neg_w_rule_sub_ptree_fit. fold neg_w_rule_sub_ptree_fit.
+      unfold formula_sub_ind_fit. fold formula_sub_ind_fit. unfold eq_f. unfold ptree_formula. unfold neg_w_rule_sub_formula. rewrite sub_fit_false; auto.
 
-- exists zero; auto. simpl. inversion Hs. rewrite neg_w_rule_simp; simpl; auto.
+- simpl. inversion Hs. rewrite neg_w_rule_simp; simpl; auto.
 
-- exists zero; auto. simpl. inversion Hs. rewrite neg_w_rule_simp; simpl; auto. 
+- simpl. inversion Hs. rewrite neg_w_rule_simp; simpl; auto. 
 
-- exists zero; auto. simpl. destruct S; inversion Hs. rewrite neg_w_rule_simp; simpl; auto.
+- simpl. destruct S; inversion Hs. rewrite neg_w_rule_simp; simpl; auto.
   unfold neg_w_rule_sub_formula. rewrite formula_sub_ind_lor; auto.
-Qed.
-
-
-Lemma neg_w_rule_ptree_formula : forall (P : ptree) (E : formula) (n : nat),
-  valid P ->
-  forall (S : subst_ind),
-    {t : term & closed_t t = true /\ ptree_formula (neg_w_rule_sub_ptree P E n t (neg_w_rule_trace P S)) =
-    neg_w_rule_sub_formula (ptree_formula P) E n t (neg_w_rule_trace P S)}.
-Proof.
-intros. destruct (subst_ind_fit (ptree_formula P) S) eqn:Hs.
-- apply neg_w_rule_ptree_formula'; auto.
-- exists zero; split; auto. apply neg_w_rule_ptree_formula_aux. apply neg_w_rule_trace_fits_not. auto.
 Defined.
 
 (* Second, we must prove that w_rule_sub_ptree does not change the degree
@@ -457,10 +523,43 @@ intros P E n t H. induction P; intros S; unfold neg_w_rule_sub_ptree.
 - simpl. destruct S; auto. destruct (subst_ind_fit f S1 && subst_ind_fit f1 S2); auto.
 Qed.
 
-(* (neg_w_rule_trace P S) *)
-
+(*
 Definition neg_w_rule_counter (P : ptree) (E : formula) (n : nat) (H : valid P) (S : subst_ind) : term := (projT1 (neg_w_rule_ptree_formula P E n H S)).
 
+Definition neg_w_rule_term (P : ptree) (E : formula) (n : nat) (H : valid P) : forall (S : subst_ind), subst_ind_fit (ptree_formula P) S = true -> term.
+induction P; intros.
+- destruct H. simpl in H0. apply (IHP v S). auto.
+- destruct H as [[X1 X2] X3]. simpl in H0. apply (IHP X2 S). auto.
+- intros. exact zero.
+- destruct H as [[[X1 X2] X3] X4]; destruct S; inversion H0; apply (IHP X2 (lor_ind S2 S1)); auto. rewrite X1. simpl. apply and_bool_symm; auto.
+- destruct H as [[[X1 X2] X3] X4]; destruct S; inversion H0; destruct S1; inversion H0; apply (IHP X2 (lor_ind (lor_ind S1_1 S2) S1_2)); auto. rewrite X1. simpl. apply and_bool_prop in H1; destruct H1. rewrite H1. apply and_bool_prop in H; destruct H. rewrite H. auto.
+- destruct H as [[[X1 X2] X3] X4]; destruct S; inversion H0; destruct S1; inversion H0; apply (IHP X2 (lor_ind (lor_ind S1_2 S1_1) S2)); auto. rewrite X1. simpl. apply and_bool_prop in H1; destruct H1. rewrite H1. apply and_bool_prop in H; destruct H. rewrite H. rewrite H3. auto.
+- destruct H as [[[X1 X2] X3] X4]; destruct S; inversion H0; destruct S1; inversion H0; destruct S1_1; inversion H0; apply (IHP X2 (lor_ind (lor_ind (lor_ind S1_1_1 S1_2) S1_1_2) S2)); auto. rewrite X1. simpl. apply and_bool_prop in H1; destruct H1. rewrite H1. apply and_bool_prop in H; destruct H. apply and_bool_prop in H; destruct H. rewrite H. rewrite H4. rewrite H5. auto.
+- destruct H as [[[X1 X2] X3] X4]; apply (IHP X2 (lor_ind S S)); auto. rewrite X1. simpl. simpl in H0. rewrite H0. auto.
+- destruct H as [[[X1 X2] X3] X4]; destruct S; inversion H0. apply (IHP X2 (lor_ind (lor_ind S1 S1) S2)); auto. rewrite X1. simpl. apply and_bool_prop in H1. destruct H1. rewrite H1. rewrite H. auto.
+- destruct H as [[[[X1 X2] X3] X4] X5]; destruct S; inversion H0; apply (IHP X3 S2); auto. rewrite X1. apply and_bool_prop in H1. destruct H1. auto.
+- destruct H as [[[[[[X1 X2] X3] X4] X5] X6] X7]; apply (IHP2 X3 S); auto. rewrite X2. destruct S; inversion H0; auto.
+- destruct H as [[[[[[X1 X2] X3] X4] X5] X6] X7]; apply (IHP2 X3 S); auto. rewrite X2. destruct S; inversion H0; auto.
+- destruct H as [[[X1 X2] X3] X4]; destruct S; inversion H0; auto. apply (IHP X2 (non_target f)); auto. rewrite X1. apply non_target_fit. apply (IHP X2 (target f)); auto. rewrite X1. apply target_fit.
+- destruct H as [[[X1 X2] X3] X4]; destruct S; inversion H0; auto; destruct S1;inversion H0. apply (IHP X2 (lor_ind (non_target f) S2)); auto. rewrite X1. simpl. rewrite non_target_fit. auto. apply (IHP X2 (lor_ind (target f) S2)); auto. rewrite X1. simpl. rewrite target_fit. auto.
+- exact (projT1 (neg_w_rule_ptree_formula (quantification_a f n0 t n1 o P) E n H S)).
+- exact (projT1 (neg_w_rule_ptree_formula (quantification_ad f f0 n0 t n1 o P) E n H S)).
+- destruct (H 0) as [[[X1 X2] X3] X4]. fold valid in X2. destruct S; inversion H0. apply (X 0 X2 (non_target f)). rewrite X1. rewrite (non_target_term_sub f n0 zero). apply non_target_fit. apply (X 0 X2 (target f)). rewrite X1. rewrite (target_term_sub f n0 zero). apply target_fit.
+- destruct (H 0) as [[[X1 X2] X3] X4]. fold valid in X2. destruct S; inversion H0. destruct S1; inversion H0. apply (X 0 X2 (lor_ind (non_target f) S2)). rewrite X1. rewrite (non_target_term_sub f n0 zero). simpl. rewrite non_target_fit. auto. apply (X 0 X2 (lor_ind (target f) S2)). rewrite X1. simpl. rewrite (target_term_sub f n0 zero). rewrite target_fit. auto.
+- destruct H as [[[[[[[X1 X2] X3] X4] X5] X6] X7] X8]; apply (IHP1 X2 (lor_ind S (non_target f0))); auto. rewrite X1. simpl. simpl in H0. rewrite H0. apply non_target_fit.
+- destruct H as [[[[[[[X1 X2] X3] X4] X5] X6] X7] X8]; apply (IHP2 X4 (lor_ind (0) S)); auto. rewrite X3. simpl. simpl in H0. apply H0.
+- destruct H as [[[[[[[X1 X2] X3] X4] X5] X6] X7] X8]; destruct S; inversion H0. apply (IHP2 X4 (lor_ind (0) S2)); auto. rewrite X3. simpl. apply and_bool_prop in H1. destruct H1. auto.
+Defined.
+*)
+
+Lemma neg_w_rule_term_inv : forall (P : ptree) (E : formula) (n : nat) (H G : valid P) (S : subst_ind), (neg_w_rule_term P E n H S) = (neg_w_rule_term P E n G S).
+Proof.
+intros P. induction P; intros.
+- simpl. destruct H,G. apply IHP.
+- simpl. destruct H,G. destruct p,p0. apply IHP.
+Admitted.
+
+(*
 Lemma neg_w_rule_counter_closed : forall (P : ptree) (E : formula) (n : nat) (H : valid P) (S : subst_ind), closed_t (neg_w_rule_counter P E n H S) = true.
 Proof.
 intros. unfold neg_w_rule_counter. destruct neg_w_rule_ptree_formula. simpl. destruct a. auto.
@@ -470,10 +569,268 @@ Lemma neg_w_rule_counter_formula : forall (P : ptree) (E : formula) (n : nat) (H
 Proof.
 intros. unfold neg_w_rule_counter. destruct neg_w_rule_ptree_formula. simpl. destruct a. auto.
 Qed.
+*)
+
 
 (* Now we prove that if we have a valid ptree, performing our
 w_rule substitution on it results in a valid ptree *)
-(* *)
+
+(*
+Lemma valid_to_formula : forall (P : ptree) (E : formula) (n : nat) (t: term) (S : subst_ind), valid (neg_w_rule_sub_ptree P E n t S) -> ptree_formula (neg_w_rule_sub_ptree P E n t (neg_w_rule_trace P S)) = neg_w_rule_sub_formula (ptree_formula P) E n t (neg_w_rule_trace P S).
+Admitted.
+*)
+
+
+(*
+Lemma neg_w_rule_valid : forall (P : ptree) (E : formula) (n : nat) (H : valid P) (S : subst_ind),
+    subst_ind_fit (ptree_formula P) S = true ->
+      {t : term & valid (neg_w_rule_sub_ptree P E n t (neg_w_rule_trace P S))}.
+Proof.
+intros P E n.
+induction P; try intros H S Hs; unfold neg_w_rule_sub_ptree.
+
+- simpl. inversion H as [H1 H2]. inversion Hs. rewrite neg_w_rule_trace_fits; auto.
+  destruct (IHP H2 S H3) as [t Ht].
+  exists t. rewrite neg_w_rule_ptree_formula_true; auto. split; simpl; auto. 
+  rewrite <- neg_w_rule_ptree_deg; auto. rewrite neg_w_rule_trace_fits; auto.
+
+- simpl. inversion H as [[H1 H2] H3]. inversion Hs. rewrite neg_w_rule_trace_fits; auto.
+  destruct (IHP H2 S Hs) as [t Ht].
+  exists t. rewrite neg_w_rule_ptree_formula_true; auto. repeat split; simpl; auto. 
+  rewrite neg_w_rule_ptree_ord; auto. rewrite neg_w_rule_trace_fits; auto.
+
+- exists zero. simpl. destruct (subst_ind_fit f S); apply H.
+
+- simpl. destruct S; inversion Hs. rewrite H1.
+  inversion H as [[[H2 H3] H4] H5].
+  assert (subst_ind_fit (ptree_formula P) (lor_ind S2 S1) = true) as Z. rewrite H2. simpl. apply and_bool_symm; auto.
+  destruct (IHP H3 (lor_ind S2 S1) Z) as [t Ht].
+  exists t. rewrite neg_w_rule_ptree_formula_true; auto. repeat split; auto.
+  + pose (valid_to_formula _ _ _ _ _ Ht). admit.
+  + admit.
+  + rewrite <- neg_w_rule_ptree_deg; auto.
+  + rewrite neg_w_rule_ptree_ord; auto.
+
+- simpl. destruct S; try destruct S1; inversion Hs.
+  rewrite H1. simpl. inversion H as [[[H4 H5] H6] H7].
+  destruct (and_bool_prop _ _ H1). clear H1.
+  destruct (and_bool_prop _ _ H0). clear H0.
+  repeat split; try rewrite neg_w_rule_ptree_formula_true.
+  + admit.
+  + rewrite H4. simpl. rewrite H1, H2, H3. auto.
+  + admit.
+  + rewrite H4. simpl. rewrite H1, H2, H3. auto.
+  + rewrite <- neg_w_rule_ptree_deg; auto.
+  + rewrite H4. simpl. rewrite H1, H2, H3. auto.
+  + rewrite neg_w_rule_ptree_ord; auto.
+  + rewrite H4. simpl. rewrite H1, H2, H3. auto.
+
+- simpl. destruct S; try destruct S1; inversion Hs.
+  rewrite H1. simpl. inversion H as [[[H4 H5] H6] H7].
+  destruct (and_bool_prop _ _ H1). clear H1.
+  destruct (and_bool_prop _ _ H0). clear H0.
+  repeat split; rewrite neg_w_rule_ptree_formula_true.
+  + admit.
+  + rewrite H4. simpl. rewrite H1, H2, H3. auto.
+  + admit.
+  + rewrite H4. simpl. rewrite H1, H2, H3. auto.
+  + rewrite <- neg_w_rule_ptree_deg; auto.
+  + rewrite H4. simpl. rewrite H1, H2, H3. auto.
+  + rewrite neg_w_rule_ptree_ord; auto.
+  + rewrite H4. simpl. rewrite H1, H2, H3. auto.
+
+- simpl. destruct S; try destruct S1; try destruct S1_1; inversion Hs.
+  rewrite H1. simpl. inversion H as [[[H5 H6] H7] H8].
+  destruct (and_bool_prop _ _ H1). clear H1.
+  destruct (and_bool_prop _ _ H0). clear H0.
+  destruct (and_bool_prop _ _ H1). clear H1.
+  repeat split; rewrite neg_w_rule_ptree_formula_true.
+  + admit.
+  + rewrite H5. simpl. rewrite H0, H2, H3, H4. auto.
+  + admit.
+  + rewrite H5. simpl. rewrite H0, H2, H3, H4. auto.
+  + rewrite <- neg_w_rule_ptree_deg; auto.
+  + rewrite H5. simpl. rewrite H0, H2, H3, H4. auto.
+  + rewrite neg_w_rule_ptree_ord; auto.
+  + rewrite H5. simpl. rewrite H0, H2, H3, H4. auto.
+
+- simpl. inversion Hs. rewrite H1. inversion H as [[[H2 H3] H4] H5].
+  repeat split; rewrite neg_w_rule_ptree_formula_true.
+  + admit.
+  + rewrite H2. simpl. rewrite H1. auto.
+  + admit.
+  + rewrite H2. simpl. rewrite H1. auto.
+  + rewrite <- neg_w_rule_ptree_deg; auto.
+  + rewrite H2. simpl. rewrite H1. auto.
+  + rewrite neg_w_rule_ptree_ord; auto.
+  + rewrite H2. simpl. rewrite H1. auto.
+
+- simpl. destruct S; inversion Hs. rewrite H1.
+  inversion H as [[[H2 H3] H4] H5]. destruct (and_bool_prop _ _ H1).
+  repeat split; rewrite neg_w_rule_ptree_formula_true.
+  + admit.
+  + rewrite H2. simpl. rewrite H0, H6. auto.
+  + admit.
+  + rewrite H2. simpl. rewrite H0, H6. auto.
+  + rewrite <- neg_w_rule_ptree_deg; auto.
+  + rewrite H2. simpl. rewrite H0, H6. auto.
+  + rewrite neg_w_rule_ptree_ord; auto.
+  + rewrite H2. simpl. rewrite H0, H6. auto.
+
+- simpl. destruct S; inversion Hs. rewrite H1. simpl.
+  inversion H as [[[[H2 H3] H4] H5] H6]. destruct (and_bool_prop _ _ H1).
+  repeat split; try rewrite neg_w_rule_ptree_formula_true; try rewrite H2; auto.
+  + admit.
+  + apply neg_w_rule_sub_formula_closed. auto. apply neg_w_rule_counter_closed.
+  + admit.
+  + rewrite <- neg_w_rule_ptree_deg; auto.
+  + rewrite neg_w_rule_ptree_ord; auto.
+
+- simpl. destruct S; apply H.
+
+- simpl. destruct S; try apply H.
+  destruct H as [[[[[[[H2 H3] H4] H5] H6] H7] H8] H9].
+  assert (subst_ind_fit (ptree_formula P1) (lor_ind (0) S2) = true) as Z. inversion Hs. rewrite H2. destruct S1; simpl; auto. inversion H0.
+  assert (subst_ind_fit (ptree_formula P1) (lor_ind (1) S2) = true) as Z1. inversion Hs. rewrite H2. destruct S1; simpl; auto. inversion H0.
+  assert (subst_ind_fit (ptree_formula P2) (lor_ind (0) S2) = true) as Z2. inversion Hs. rewrite H4. destruct S1; simpl; auto. inversion H0.
+  assert (subst_ind_fit (ptree_formula P2) (lor_ind (1) S2) = true) as Z3. inversion Hs. rewrite H4. destruct S1; simpl; auto. inversion H0.
+  destruct S1; inversion Hs; rewrite H0; simpl.
+  + repeat split; rewrite neg_w_rule_ptree_formula_true; auto.
+    * admit.
+    * admit.
+    * admit.
+    * admit.
+    * rewrite H6. rewrite <- neg_w_rule_ptree_deg; auto.
+    * rewrite H7. rewrite <- neg_w_rule_ptree_deg; auto.
+    * rewrite neg_w_rule_ptree_ord; auto.
+    * rewrite neg_w_rule_ptree_ord; auto.
+  + repeat split; rewrite neg_w_rule_ptree_formula_true; auto.
+    * admit.
+    * admit.
+    * admit.
+    * admit.
+    * rewrite H6. rewrite <- neg_w_rule_ptree_deg; auto.
+    * rewrite H7. rewrite <- neg_w_rule_ptree_deg; auto.
+    * rewrite neg_w_rule_ptree_ord; auto.
+    * rewrite neg_w_rule_ptree_ord; auto.
+
+- simpl. destruct S; destruct (eq_f f E); apply H.
+
+- simpl. inversion H as [[[H1 H2] H3] H4]. destruct S; auto.
+  destruct S1; auto; destruct (subst_ind_fit f0 S2) eqn:HS2; simpl;
+  repeat split; auto; rewrite neg_w_rule_ptree_formula_true;
+  try apply IHP; auto; try rewrite H1; simpl; try rewrite non_target_fit,HS2;
+  try rewrite w_rule_ptree_deg; try rewrite w_rule_ptree_ord; auto.
+  + admit.
+  + admit.
+  + rewrite <- neg_w_rule_ptree_deg; auto.
+  + rewrite neg_w_rule_ptree_ord; auto.
+  + admit.
+  + admit.
+  + rewrite <- neg_w_rule_ptree_deg; auto.
+  + rewrite neg_w_rule_ptree_ord; auto.
+
+- simpl. inversion H as [[[[H0 H1] H2] H3] H4]. destruct S; auto; case (eq_f f E) eqn:X; case (eq_nat n0 n) eqn:X1; case (eq_term (neg_w_rule_counter (quantification_a f n0 t n1 o P) E n H (0)) t) eqn:X2; case (eq_term (neg_w_rule_counter (quantification_a f n0 t n1 o P) E n H (1)) t) eqn:X3; simpl; auto; repeat split; auto; rewrite H4; try apply ord_succ_monot; auto; apply ord_succ_nf; apply ptree_ord_nf; auto.
+
+- simpl. destruct S; try apply H. inversion H as [[[[H0 H1] H2] H3] H4].
+  assert (subst_ind_fit (ptree_formula P) (lor_ind (0) S2) = true). rewrite H0. simpl. destruct S1; inversion Hs; rewrite H6; auto.
+  assert (subst_ind_fit (ptree_formula P) (lor_ind (1) S2) = true). rewrite H0. simpl. destruct S1; inversion Hs; rewrite H7; auto.
+  destruct S1; inversion Hs; simpl; auto; rewrite neg_w_rule_ptree_formula_true; try rewrite H7; try rewrite H8; auto; simpl; repeat split; auto.
+  + case (eq_f f E).
+    * case (eq_nat n0 n).
+      --  case (eq_term (neg_w_rule_counter (quantification_ad f f0 n0 t n1 o P) E n H (lor_ind (0) S2)) t).
+          ++ repeat split; auto.
+             **  admit.
+             **  apply neg_w_rule_counter_closed.
+             **  admit.
+             **  rewrite <- neg_w_rule_ptree_deg; auto.
+             **  rewrite neg_w_rule_ptree_ord; auto.
+          ++  repeat split; auto.
+              **  admit.
+              **  apply neg_w_rule_counter_closed.
+              **  admit.
+              **  rewrite <- neg_w_rule_ptree_deg; auto.
+              **  rewrite neg_w_rule_ptree_ord; auto.
+      --  repeat split; auto.
+          ++  admit.
+          ++  apply neg_w_rule_counter_closed.
+          ++  admit.
+          ++  rewrite <- neg_w_rule_ptree_deg; auto.
+          ++  rewrite neg_w_rule_ptree_ord; auto.
+    * repeat split; auto.
+      --  admit.
+      --  apply neg_w_rule_counter_closed.
+      --  admit.
+      --  rewrite <- neg_w_rule_ptree_deg; auto.
+      --  rewrite neg_w_rule_ptree_ord; auto.
+    + case (eq_f f E).
+      * case (eq_nat n0 n).
+        --  case (eq_term (neg_w_rule_counter (quantification_ad f f0 n0 t n1 o P) E n H (lor_ind (1) S2)) t).
+            ++ repeat split; auto; rewrite H4. apply ord_succ_monot. apply ord_succ_nf. apply ptree_ord_nf; auto.
+            ++  repeat split; auto.
+                **  admit.
+                **  apply neg_w_rule_counter_closed.
+                **  admit.
+                **  rewrite <- neg_w_rule_ptree_deg; auto.
+                **  rewrite neg_w_rule_ptree_ord; auto.
+        --  repeat split; auto.
+            ++  admit.
+            ++  apply neg_w_rule_counter_closed.
+            ++  admit.
+            ++  rewrite <- neg_w_rule_ptree_deg; auto.
+            ++  rewrite neg_w_rule_ptree_ord; auto.
+      * repeat split; auto.
+        --  admit.
+        --  apply neg_w_rule_counter_closed.
+        --  admit.
+        --  rewrite <- neg_w_rule_ptree_deg; auto.
+        --  rewrite neg_w_rule_ptree_ord; auto.
+    
+
+- rewrite Hs. simpl. intros. destruct (H m) as [[[H1 H2] H3] H4]. fold valid in H2. repeat split; auto.
+
+- rewrite Hs. simpl. destruct S; inversion Hs. simpl; intros; destruct (H m) as [[[X1 X2] X3] X4]; fold valid in X2; assert (subst_ind_fit (ptree_formula (p m)) (lor_ind (non_target f) S2) = true). rewrite X1. simpl. destruct S1; inversion Hs; rewrite H2; rewrite (non_target_term_sub f n0 (represent m)); rewrite non_target_fit; auto. destruct S1; inversion Hs; simpl; auto; rewrite neg_w_rule_ptree_formula_true; auto; repeat split; auto.
+  + admit.
+  + admit.
+  + rewrite <- neg_w_rule_ptree_deg; auto.
+  + rewrite neg_w_rule_ptree_ord; auto.
+  + admit.
+  + admit.
+  + rewrite <- neg_w_rule_ptree_deg; auto.
+  + rewrite neg_w_rule_ptree_ord; auto. 
+
+- clear IHP2. rewrite Hs. inversion H as [[[[[[[H1 H2] H3] H4] H5] H6] H7] H8]. inversion Hs. assert (subst_ind_fit (ptree_formula P1) (lor_ind S (non_target f0)) = true). rewrite H1. simpl. rewrite H9. rewrite non_target_fit. auto.
+  repeat split; auto; rewrite neg_w_rule_ptree_formula_true; auto.
+  + admit.
+  + admit.
+  + rewrite <- neg_w_rule_ptree_deg; auto.
+  + rewrite neg_w_rule_ptree_ord; auto.
+
+- clear IHP1. rewrite Hs. inversion H as [[[[[[[H1 H2] H3] H4] H5] H6] H7] H8]. inversion Hs. assert (subst_ind_fit (ptree_formula P2) (lor_ind (0) S) = true). rewrite H3. simpl. rewrite H9. auto.
+  repeat split; auto; rewrite neg_w_rule_ptree_formula_true; auto.
+  + admit.
+  + admit.
+  + rewrite <- neg_w_rule_ptree_deg; auto.
+  + rewrite neg_w_rule_ptree_ord; auto.
+
+- rewrite Hs. inversion H as [[[[[[[H1 H2] H3] H4] H5] H6] H7] H8].
+  destruct S; try inversion Hs.
+  destruct (and_bool_prop _ _ H9) as [H10 H11].
+  assert (subst_ind_fit (ptree_formula P1) (lor_ind S1 (non_target f0)) = true). rewrite H1. simpl. rewrite H10. rewrite non_target_fit. auto.
+  assert (subst_ind_fit (ptree_formula P2) (lor_ind (0) S2) = true). rewrite H3. simpl. rewrite H11. auto.
+  simpl. repeat split; rewrite neg_w_rule_ptree_formula_true; auto.
+  + admit.
+  + admit.
+  + admit.
+  + admit.
+  + rewrite <- neg_w_rule_ptree_deg; auto.
+  + rewrite <- neg_w_rule_ptree_deg; auto.
+  + rewrite neg_w_rule_ptree_ord; auto.
+  + rewrite neg_w_rule_ptree_ord; auto.
+Admitted.
+
+*)
+(*
 Lemma neg_w_rule_valid : forall (P : ptree) (E : formula) (n : nat) (H : valid P) (S : subst_ind),
     subst_ind_fit (ptree_formula P) S = true ->
       valid (neg_w_rule_sub_ptree P E n (neg_w_rule_counter P E n H S) S).
@@ -484,7 +841,13 @@ induction P; try intros H S Hs; unfold neg_w_rule_sub_ptree.
 - simpl. inversion H as [H1 H2]. inversion Hs. rewrite H3.
   pose proof (IHP H2 S H3) as Ht.
   rewrite neg_w_rule_ptree_formula_true; auto. split; simpl; auto. 
-  rewrite <- neg_w_rule_ptree_deg; auto. admit.
+  rewrite <- neg_w_rule_ptree_deg; auto.
+  
+  unfold neg_w_rule_counter in *.
+  unfold neg_w_rule_ptree_formula in *. unfold ptree_formula in *. fold ptree_formula in *.
+  unfold neg_w_rule_trace in *. fold neg_w_rule_trace in *. unfold neg_w_rule_sub_ptree in *. rewrite H3 at 1. rewrite H3 in Ht at 1. apply Ht.
+  simpl. destruct H. destruct (neg_w_rule_ptree_formula' P E n v S Hs0). apply Ht.
+  unfold neg_w_rule_ptree_formula'.
 
 - simpl. inversion H as [[H1 H2] H3]. inversion Hs. rewrite H4.
   pose proof (IHP H2 S Hs) as Ht.
@@ -610,264 +973,369 @@ induction P; try intros H S Hs; unfold neg_w_rule_sub_ptree.
 
 - simpl. inversion H as [[[H1 H2] H3] H4]. destruct S; auto.
   destruct S1; auto; destruct (subst_ind_fit f0 S2) eqn:HS2; simpl;
-  repeat split; auto; rewrite w_rule_ptree_formula_true;
+  repeat split; auto; rewrite neg_w_rule_ptree_formula_true;
   try apply IHP; auto; try rewrite H1; simpl; try rewrite non_target_fit,HS2;
   try rewrite w_rule_ptree_deg; try rewrite w_rule_ptree_ord; auto.
-  + rewrite w_rule_ptree_formula; auto. rewrite H1.
-    unfold w_rule_sub_formula. simpl. rewrite non_target_fit,HS2.
-    simpl. rewrite <- sub_fit_true; auto.
-    * rewrite non_target_sub. rewrite <- sub_fit_true; auto.
-    * apply non_target_fit.
-  + rewrite H3. apply w_rule_ptree_deg; auto.
-  + rewrite w_rule_ptree_formula; auto. rewrite H1.
-    unfold w_rule_sub_formula. simpl. rewrite non_target_fit,HS2.
-    simpl. rewrite <- sub_fit_true; auto.
-    * rewrite non_target_sub. rewrite <- sub_fit_true; auto.
-    * apply non_target_fit.
-  + rewrite H3. apply w_rule_ptree_deg; auto.
+  + admit.
+  + admit.
+  + rewrite <- neg_w_rule_ptree_deg; auto.
+  + rewrite neg_w_rule_ptree_ord; auto.
+  + admit.
+  + admit.
+  + rewrite <- neg_w_rule_ptree_deg; auto.
+  + rewrite neg_w_rule_ptree_ord; auto.
 
-- simpl. destruct S; auto.
+- simpl. inversion H as [[[[H0 H1] H2] H3] H4]. destruct S; auto; case (eq_f f E) eqn:X; case (eq_nat n0 n) eqn:X1; case (eq_term (neg_w_rule_counter (quantification_a f n0 t n1 o P) E n H (0)) t) eqn:X2; case (eq_term (neg_w_rule_counter (quantification_a f n0 t n1 o P) E n H (1)) t) eqn:X3; simpl; auto; repeat split; auto; rewrite H4; try apply ord_succ_monot; auto; apply ord_succ_nf; apply ptree_ord_nf; auto.
 
 - simpl. destruct S; try apply H. inversion H as [[[[H0 H1] H2] H3] H4].
-  destruct S1; inversion Hs; rewrite H6; simpl.
-  + repeat split; auto.
-    * rewrite w_rule_ptree_formula_true, w_rule_ptree_formula; auto.
-      { rewrite H0. unfold w_rule_sub_formula.
-        { rewrite formula_sub_ind_lor. simpl.
-          { destruct (eq_f (substitution f n t)); auto. }
-          { simpl. apply H6. } } }
-      { rewrite H0. simpl. apply H6. }
-    * rewrite w_rule_ptree_formula_true.
-      { apply IHP; auto. rewrite H0. simpl. apply H6. }
-      { rewrite H0. simpl. apply H6. }
-    * rewrite w_rule_ptree_formula_true.
-      { rewrite H3. apply w_rule_ptree_deg; auto. }
-      { rewrite H0. simpl. auto. }
-    * rewrite w_rule_ptree_formula_true.
-      { rewrite w_rule_ptree_ord; auto. }
-      { rewrite H0. simpl. auto. }
-  + repeat split; auto.
-    * rewrite w_rule_ptree_formula_true, w_rule_ptree_formula; auto.
-      { rewrite H0. unfold w_rule_sub_formula.
-        { rewrite formula_sub_ind_lor. simpl.
-          { destruct (eq_f (substitution f n t)); auto. }
-          { simpl. apply H6. } } }
-      { rewrite H0. simpl. apply H6. }
-    * rewrite w_rule_ptree_formula_true.
-      { apply IHP; auto. rewrite H0. simpl. apply H6. }
-      { rewrite H0. simpl. apply H6. }
-    * rewrite w_rule_ptree_formula_true.
-      { rewrite H3. apply w_rule_ptree_deg; auto. }
-      { rewrite H0. simpl. auto. }
-    * rewrite w_rule_ptree_formula_true.
-      { rewrite w_rule_ptree_ord; auto. }
-      { rewrite H0. simpl. auto. }
+  assert (subst_ind_fit (ptree_formula P) (lor_ind (0) S2) = true). rewrite H0. simpl. destruct S1; inversion Hs; rewrite H6; auto.
+  assert (subst_ind_fit (ptree_formula P) (lor_ind (1) S2) = true). rewrite H0. simpl. destruct S1; inversion Hs; rewrite H7; auto.
+  destruct S1; inversion Hs; simpl; auto; rewrite neg_w_rule_ptree_formula_true; try rewrite H7; try rewrite H8; auto; simpl; repeat split; auto.
+  + case (eq_f f E).
+    * case (eq_nat n0 n).
+      --  case (eq_term (neg_w_rule_counter (quantification_ad f f0 n0 t n1 o P) E n H (lor_ind (0) S2)) t).
+          ++ repeat split; auto.
+             **  admit.
+             **  apply neg_w_rule_counter_closed.
+             **  admit.
+             **  rewrite <- neg_w_rule_ptree_deg; auto.
+             **  rewrite neg_w_rule_ptree_ord; auto.
+          ++  repeat split; auto.
+              **  admit.
+              **  apply neg_w_rule_counter_closed.
+              **  admit.
+              **  rewrite <- neg_w_rule_ptree_deg; auto.
+              **  rewrite neg_w_rule_ptree_ord; auto.
+      --  repeat split; auto.
+          ++  admit.
+          ++  apply neg_w_rule_counter_closed.
+          ++  admit.
+          ++  rewrite <- neg_w_rule_ptree_deg; auto.
+          ++  rewrite neg_w_rule_ptree_ord; auto.
+    * repeat split; auto.
+      --  admit.
+      --  apply neg_w_rule_counter_closed.
+      --  admit.
+      --  rewrite <- neg_w_rule_ptree_deg; auto.
+      --  rewrite neg_w_rule_ptree_ord; auto.
+    + case (eq_f f E).
+      * case (eq_nat n0 n).
+        --  case (eq_term (neg_w_rule_counter (quantification_ad f f0 n0 t n1 o P) E n H (lor_ind (1) S2)) t).
+            ++ repeat split; auto; rewrite H4. apply ord_succ_monot. apply ord_succ_nf. apply ptree_ord_nf; auto.
+            ++  repeat split; auto.
+                **  admit.
+                **  apply neg_w_rule_counter_closed.
+                **  admit.
+                **  rewrite <- neg_w_rule_ptree_deg; auto.
+                **  rewrite neg_w_rule_ptree_ord; auto.
+        --  repeat split; auto.
+            ++  admit.
+            ++  apply neg_w_rule_counter_closed.
+            ++  admit.
+            ++  rewrite <- neg_w_rule_ptree_deg; auto.
+            ++  rewrite neg_w_rule_ptree_ord; auto.
+      * repeat split; auto.
+        --  admit.
+        --  apply neg_w_rule_counter_closed.
+        --  admit.
+        --  rewrite <- neg_w_rule_ptree_deg; auto.
+        --  rewrite neg_w_rule_ptree_ord; auto.
+    
 
-- rename f into A. rename p into g. rename n1 into d. rename o into alpha.
-  destruct (valid_w_rule_a A n0 d alpha g H m) as [[[H1 H2] H3] H4].
-  simpl. destruct S; auto;
-  destruct (eq_nat d (ptree_deg (g m))) eqn:HD; destruct (eq_f A E) eqn:HE; auto; destruct (eq_nat n0 n) eqn:Hn; simpl; auto; repeat split; auto.
-  rewrite H4. apply omega_exp_incr.
-  apply single_nf. rewrite H4. apply (ptree_ord_nf (g m) H2).
-  apply leq_type in H3. destruct H3 as [H3 | H3]. auto. rewrite H3 in HD. rewrite eq_nat_refl in HD. inversion HD.
-  rewrite H4. apply omega_exp_incr.
-  apply single_nf. rewrite H4. apply (ptree_ord_nf (g m) H2).
+- rewrite Hs. simpl. intros. destruct (H m) as [[[H1 H2] H3] H4]. fold valid in H2. repeat split; auto.
 
-- rename f into A. rename f0 into D. rename p into g.
-  rename n1 into d. rename o into alpha.
-  simpl. destruct S; auto. destruct S1; auto.
-  + destruct (eq_nat d (ptree_deg (g m))) eqn:HD.
-    * destruct (eq_f A E) eqn:HE.
-      { destruct (subst_ind_fit D S2) eqn:HS2; simpl.
-        { destruct (eq_nat n0 n) eqn:Hn; simpl; intros p;
-          destruct (valid_w_rule_ad A D n0 d alpha g H p) as [[[H1 H2] H3] H4].
-          { repeat split; rewrite w_rule_ptree_formula_true;
-            try rewrite w_rule_ptree_deg; try rewrite w_rule_ptree_ord; auto;
-            try rewrite w_rule_ptree_formula; try apply X; auto;
-            try rewrite H1; simpl; try rewrite (non_target_term_sub A n0 (represent p));
-            try rewrite non_target_fit,HS2; auto;
-            unfold w_rule_sub_formula; try rewrite non_target_sub_lor; auto.
-            pose proof (w_rule_ptree_deg (g p) E n m H2 (lor_ind (non_target (substitution A n0 (represent p))) S2 )). lia. }
-          { repeat split; rewrite w_rule_ptree_formula_true;
-          try rewrite w_rule_ptree_deg; try rewrite w_rule_ptree_ord; auto;
-          try rewrite w_rule_ptree_formula; try apply X; auto;
-          try rewrite H1; simpl; try rewrite (non_target_term_sub A n0 (represent p));
-          try rewrite non_target_fit,HS2; auto;
-          unfold w_rule_sub_formula; try rewrite non_target_sub_lor; auto.
-          pose proof (w_rule_ptree_deg (g p) E n m H2 (lor_ind (non_target (substitution A n0 (represent p))) S2 )). lia. } }
-        { destruct (eq_nat n0 n) eqn:Hn; simpl; intros p;
-          destruct (valid_w_rule_ad A D n0 d alpha g H p) as [[[H1 H2] H3] H4];
-          repeat split; auto. } }
-      { destruct (subst_ind_fit D S2) eqn:HS2; simpl; intro p;
-        destruct (valid_w_rule_ad A D n0 d alpha g H p) as [[[H1 H2] H3] H4];
-        repeat split; auto; rewrite w_rule_ptree_formula_true;
-        try rewrite w_rule_ptree_deg; try rewrite w_rule_ptree_ord; auto;
-        try rewrite w_rule_ptree_formula; try apply X; auto;
-        try rewrite H1; simpl; rewrite (non_target_term_sub A n0 (represent p));
-        try rewrite non_target_fit,HS2; auto.
-        unfold w_rule_sub_formula. rewrite non_target_sub_lor. auto.
-        pose proof (w_rule_ptree_deg (g p) E n m H2 (lor_ind (non_target (substitution A n0 (represent p))) S2 )). lia. }
-    * destruct (eq_f A E) eqn:HE.
-      { destruct (subst_ind_fit D S2) eqn:HS2; simpl.
-        { destruct (eq_nat n0 n) eqn:Hn; simpl; intros p;
-          destruct (valid_w_rule_ad A D n0 d alpha g H p) as [[[H1 H2] H3] H4].
-          { repeat split; rewrite w_rule_ptree_formula_true;
-            try rewrite w_rule_ptree_deg; try rewrite w_rule_ptree_ord; auto;
-            try rewrite w_rule_ptree_formula; try apply X; auto;
-            try rewrite H1; simpl; try rewrite (non_target_term_sub A n0 (represent p));
-            try rewrite non_target_fit,HS2; auto;
-            unfold w_rule_sub_formula; try rewrite non_target_sub_lor; auto.
-            pose proof (w_rule_ptree_deg (g p) E n m H2 (lor_ind (non_target (substitution A n0 (represent p))) S2 )). lia. }
-          { repeat split; rewrite w_rule_ptree_formula_true;
-          try rewrite w_rule_ptree_deg; try rewrite w_rule_ptree_ord; auto;
-          try rewrite w_rule_ptree_formula; try apply X; auto;
-          try rewrite H1; simpl; try rewrite (non_target_term_sub A n0 (represent p));
-          try rewrite non_target_fit,HS2; auto;
-          unfold w_rule_sub_formula; try rewrite non_target_sub_lor; auto.
-          pose proof (w_rule_ptree_deg (g p) E n m H2 (lor_ind (non_target (substitution A n0 (represent p))) S2 )). lia. } }
-        { destruct (eq_nat n0 n) eqn:Hn; simpl; intros p;
-          destruct (valid_w_rule_ad A D n0 d alpha g H p) as [[[H1 H2] H3] H4];
-          repeat split; auto. } }
-      { destruct (subst_ind_fit D S2) eqn:HS2; simpl; intro p;
-        destruct (valid_w_rule_ad A D n0 d alpha g H p) as [[[H1 H2] H3] H4];
-        repeat split; auto; rewrite w_rule_ptree_formula_true;
-        try rewrite w_rule_ptree_deg; try rewrite w_rule_ptree_ord; auto;
-        try rewrite w_rule_ptree_formula; try apply X; auto;
-        try rewrite H1; simpl; rewrite (non_target_term_sub A n0 (represent p));
-        try rewrite non_target_fit,HS2; auto.
-        unfold w_rule_sub_formula. rewrite non_target_sub_lor. auto.
-        pose proof (w_rule_ptree_deg (g p) E n m H2 (lor_ind (non_target (substitution A n0 (represent p))) S2 )). lia. }
-  + destruct (eq_nat d (ptree_deg (g m))) eqn:HD.
-    * destruct (eq_f A E) eqn:HE.
-      { destruct (subst_ind_fit D S2) eqn:HS2.
-        { simpl. destruct (eq_nat n0 n) eqn:Hn.
-          { destruct (valid_w_rule_ad A D n0 d alpha g H m) as [[[H1 H2] H3] H4].
-            unfold valid. fold valid. repeat split.
-            { rewrite <- w_rule_simp.
-              rewrite (w_rule_ptree_ord (g m) E n m H2 (lor_ind (non_target A) S2)).
-              rewrite H4. apply omega_exp_incr. 
-              rewrite H1. simpl. rewrite HS2. rewrite (non_target_term_sub _ n0 (represent m)). rewrite non_target_fit. auto. }
-            { rewrite w_rule_ptree_formula_true; try apply X; auto;
-              rewrite H1; simpl; rewrite (non_target_term_sub A n0 (represent m));
-              rewrite non_target_fit,HS2; auto. }
-            { rewrite H4. apply single_nf. apply ptree_ord_nf. auto. } }
-          { simpl. intro p.
-            destruct (valid_w_rule_ad A D n0 d alpha g H p) as [[[H1 H2] H3] H4].
-            repeat split; rewrite w_rule_ptree_formula_true;
-            try rewrite w_rule_ptree_deg; try rewrite w_rule_ptree_ord; auto;
-            try rewrite w_rule_ptree_formula; try apply X; auto;
-            try rewrite H1; simpl; rewrite (non_target_term_sub A n0 (represent p));
-            try rewrite non_target_fit,HS2; auto.
-            unfold w_rule_sub_formula. rewrite non_target_sub_lor. auto. 
-            pose proof (w_rule_ptree_deg (g p) E n m H2 (lor_ind (non_target (substitution A n0 (represent p))) S2 )). lia. } }
-        { simpl. intro p.
-          destruct (valid_w_rule_ad A D n0 d alpha g H p) as [[[H1 H2] H3] H4].
-          repeat split; auto. } }
-      { destruct (subst_ind_fit D S2) eqn:HS2; simpl; intro p;
-        destruct (valid_w_rule_ad A D n0 d alpha g H p) as [[[H1 H2] H3] H4];
-        repeat split; auto; rewrite w_rule_ptree_formula_true;
-        try rewrite w_rule_ptree_deg; try rewrite w_rule_ptree_ord; auto;
-        try rewrite w_rule_ptree_formula; try apply X; auto;
-        try rewrite H1; simpl; rewrite (non_target_term_sub A n0 (represent p));
-        try rewrite non_target_fit,HS2; auto.
-        unfold w_rule_sub_formula. rewrite non_target_sub_lor. auto.
-        pose proof (w_rule_ptree_deg (g p) E n m H2 (lor_ind (non_target (substitution A n0 (represent p))) S2 )). lia. }
-    * destruct (eq_f A E) eqn:HE.
-      { destruct (subst_ind_fit D S2) eqn:HS2.
-        { simpl. destruct (eq_nat n0 n) eqn:Hn.
-          { destruct (valid_w_rule_ad A D n0 d alpha g H m) as [[[H1 H2] H3] H4].
-            apply leq_type in H3. destruct H3 as [H3 | H3].
-            { rewrite w_rule_ptree_formula_true.
-              { simpl. repeat split.
-                { rewrite <- (w_rule_ptree_deg (g m) E n m H2 (lor_ind (non_target A) S2)). auto. }
-                { rewrite (w_rule_ptree_ord (g m) E n m H2 (lor_ind (non_target A) S2)).
-                  rewrite H4. apply omega_exp_incr. }
-                { apply X. auto. rewrite H1. simpl. rewrite (non_target_term_sub A n0 (represent m)).
-                  rewrite non_target_fit,HS2. auto. }
-                { rewrite H4. apply single_nf. apply ptree_ord_nf. auto. } }
-              { rewrite H1. simpl. rewrite (non_target_term_sub A n0 (represent m)).
-                rewrite non_target_fit,HS2. auto. } }
-            { rewrite H3 in HD. rewrite eq_nat_refl in HD. inversion HD. } }
-          { simpl. intro p.
-            destruct (valid_w_rule_ad A D n0 d alpha g H p) as [[[H1 H2] H3] H4].
-            repeat split; rewrite w_rule_ptree_formula_true;
-            try rewrite w_rule_ptree_deg; try rewrite w_rule_ptree_ord; auto;
-            try rewrite w_rule_ptree_formula; try apply X; auto;
-            try rewrite H1; simpl; rewrite (non_target_term_sub A n0 (represent p));
-            try rewrite non_target_fit,HS2; auto.
-            unfold w_rule_sub_formula. rewrite non_target_sub_lor. auto. 
-            pose proof (w_rule_ptree_deg (g p) E n m H2 (lor_ind (non_target (substitution A n0 (represent p))) S2 )). lia. } }
-        { simpl. intro p.
-          destruct (valid_w_rule_ad A D n0 d alpha g H p) as [[[H1 H2] H3] H4].
-          repeat split; auto. } }
-      { destruct (subst_ind_fit D S2) eqn:HS2; simpl; intro p;
-        destruct (valid_w_rule_ad A D n0 d alpha g H p) as [[[H1 H2] H3] H4];
-        repeat split; auto; rewrite w_rule_ptree_formula_true;
-        try rewrite w_rule_ptree_deg; try rewrite w_rule_ptree_ord; auto;
-        try rewrite w_rule_ptree_formula; try apply X; auto;
-        try rewrite H1; simpl; rewrite (non_target_term_sub A n0 (represent p));
-        try rewrite non_target_fit,HS2; auto.
-        unfold w_rule_sub_formula. rewrite non_target_sub_lor. auto.
-        pose proof (w_rule_ptree_deg (g p) E n m H2 (lor_ind (non_target (substitution A n0 (represent p))) S2 )). lia. }
+- rewrite Hs. simpl. destruct S; inversion Hs. simpl; intros; destruct (H m) as [[[X1 X2] X3] X4]; fold valid in X2; assert (subst_ind_fit (ptree_formula (p m)) (lor_ind (non_target f) S2) = true). rewrite X1. simpl. destruct S1; inversion Hs; rewrite H2; rewrite (non_target_term_sub f n0 (represent m)); rewrite non_target_fit; auto. destruct S1; inversion Hs; simpl; auto; rewrite neg_w_rule_ptree_formula_true; auto; repeat split; auto.
+  + admit.
+  + admit.
+  + rewrite <- neg_w_rule_ptree_deg; auto.
+  + rewrite neg_w_rule_ptree_ord; auto.
+  + admit.
+  + admit.
+  + rewrite <- neg_w_rule_ptree_deg; auto.
+  + rewrite neg_w_rule_ptree_ord; auto. 
 
-- clear IHP2. simpl. destruct (subst_ind_fit f S) eqn:Heq; try apply H. simpl.
-  inversion H as [[[[[[[H1 H2] H3] H4] H5] H6] H7] H8].
-  repeat split; auto; rewrite w_rule_ptree_formula_true.
-  + rewrite w_rule_ptree_formula; auto.
-    rewrite H1. unfold w_rule_sub_formula. rewrite formula_sub_ind_lor.
-    * rewrite non_target_sub. auto.
-    * rewrite Heq, non_target_fit. auto.
-  + rewrite H1. simpl. rewrite Heq, non_target_fit. auto.
-  + apply IHP1; auto. rewrite H1. simpl. rewrite Heq, non_target_fit. auto.
-  + rewrite H1. simpl. rewrite Heq, non_target_fit. auto.
-  + rewrite H5. apply w_rule_ptree_deg; auto.
-  + rewrite H1. simpl. rewrite Heq, non_target_fit. auto.
-  + rewrite w_rule_ptree_ord; auto.
-  + rewrite H1. simpl. rewrite Heq, non_target_fit. auto.
+- clear IHP2. rewrite Hs. inversion H as [[[[[[[H1 H2] H3] H4] H5] H6] H7] H8]. inversion Hs. assert (subst_ind_fit (ptree_formula P1) (lor_ind S (non_target f0)) = true). rewrite H1. simpl. rewrite H9. rewrite non_target_fit. auto.
+  repeat split; auto; rewrite neg_w_rule_ptree_formula_true; auto.
+  + admit.
+  + admit.
+  + rewrite <- neg_w_rule_ptree_deg; auto.
+  + rewrite neg_w_rule_ptree_ord; auto.
 
-- clear IHP1. simpl. destruct (subst_ind_fit f0 S) eqn:Heq; try apply H. simpl.
-  inversion H as [[[[[[[H1 H2] H3] H4] H5] H6] H7] H8].
-  repeat split; auto; rewrite w_rule_ptree_formula_true.
-  + rewrite w_rule_ptree_formula; auto.
-    rewrite H3. unfold w_rule_sub_formula. rewrite formula_sub_ind_lor.
-    * rewrite non_target_sub. auto.
-    * rewrite Heq, non_target_fit. auto.
-  + rewrite H3. simpl. auto.
-  + apply IHP2; auto. rewrite H3. simpl. auto.
-  + rewrite H3. simpl. auto.
-  + rewrite H6. apply w_rule_ptree_deg; auto.
-  + rewrite H3. simpl. auto.
-  + rewrite w_rule_ptree_ord; auto.
-  + rewrite H3. simpl. auto.
+- clear IHP1. rewrite Hs. inversion H as [[[[[[[H1 H2] H3] H4] H5] H6] H7] H8]. inversion Hs. assert (subst_ind_fit (ptree_formula P2) (lor_ind (0) S) = true). rewrite H3. simpl. rewrite H9. auto.
+  repeat split; auto; rewrite neg_w_rule_ptree_formula_true; auto.
+  + admit.
+  + admit.
+  + rewrite <- neg_w_rule_ptree_deg; auto.
+  + rewrite neg_w_rule_ptree_ord; auto.
 
-- simpl. inversion H as [[[[[[[H1 H2] H3] H4] H5] H6] H7] H8].
-  destruct S; try inversion Hs. rewrite H9.
+- rewrite Hs. inversion H as [[[[[[[H1 H2] H3] H4] H5] H6] H7] H8].
+  destruct S; try inversion Hs.
   destruct (and_bool_prop _ _ H9) as [H10 H11].
-  simpl. repeat split; rewrite w_rule_ptree_formula_true.
-  + rewrite w_rule_ptree_formula; auto.
-    rewrite H1. unfold w_rule_sub_formula. rewrite formula_sub_ind_lor.
-    * rewrite non_target_sub. auto.
-    * rewrite H10, non_target_fit. auto.
-  + rewrite H1. simpl. rewrite H10, non_target_fit. auto.
-  + apply IHP1; auto. rewrite H1. simpl. rewrite H10, non_target_fit. auto.
-  + rewrite H1. simpl. rewrite H10, non_target_fit. auto.
-  + rewrite w_rule_ptree_formula; auto.
-    rewrite H3. unfold w_rule_sub_formula. rewrite formula_sub_ind_lor.
-    * rewrite non_target_sub. auto.
-    * rewrite H11, non_target_fit. auto.
-  + rewrite H3. simpl. auto.
-  + apply IHP2; auto. rewrite H3. simpl. auto.
-  + rewrite H3. simpl. auto.
-  + rewrite H5. apply w_rule_ptree_deg; auto.
-  + rewrite H1. simpl. rewrite H10, non_target_fit. auto.
-  + rewrite H6. apply w_rule_ptree_deg; auto.
-  + rewrite H3. simpl. auto.
-  + rewrite w_rule_ptree_ord; auto.
-  + rewrite H1. simpl. rewrite H10, non_target_fit. auto.
-  + rewrite w_rule_ptree_ord; auto.
-  + rewrite H3. simpl. auto.
-Qed.
+  assert (subst_ind_fit (ptree_formula P1) (lor_ind S1 (non_target f0)) = true). rewrite H1. simpl. rewrite H10. rewrite non_target_fit. auto.
+  assert (subst_ind_fit (ptree_formula P2) (lor_ind (0) S2) = true). rewrite H3. simpl. rewrite H11. auto.
+  simpl. repeat split; rewrite neg_w_rule_ptree_formula_true; auto.
+  + admit.
+  + admit.
+  + admit.
+  + admit.
+  + rewrite <- neg_w_rule_ptree_deg; auto.
+  + rewrite <- neg_w_rule_ptree_deg; auto.
+  + rewrite neg_w_rule_ptree_ord; auto.
+  + rewrite neg_w_rule_ptree_ord; auto.
+Admitted.
+*)
 
+Arguments neg_w_rule_sub_ptree : simpl nomatch.
+
+(*Arguments neg_w_rule_term : simpl nomatch.*)
+
+
+Lemma neg_w_rule_valid_3 : forall (P : ptree) (E : formula) (n : nat) (H : valid P) (S : subst_ind) (Hs : subst_ind_fit (ptree_formula P) S = true),
+      valid (neg_w_rule_sub_ptree P E n (neg_w_rule_term P E n H S Hs) S).
+Proof.
+intros P E n.
+induction P; try intros H S Hs; unfold neg_w_rule_sub_ptree.
+
+- simpl. destruct H as [H1 H2]. inversion Hs. rewrite H0.
+  pose proof (IHP H2 S H0) as Ht.
+  rewrite neg_w_rule_ptree_formula_true; auto. split; simpl; auto. 
+  rewrite <- neg_w_rule_ptree_deg; auto.
+
+- simpl. destruct H as [[H1 H2] H3]. inversion Hs. rewrite H0.
+  pose proof (IHP H2 S Hs) as Ht.
+  rewrite neg_w_rule_ptree_formula_true; auto. repeat split; simpl; auto. 
+  rewrite neg_w_rule_ptree_ord; auto.
+
+- simpl. destruct (subst_ind_fit f S); apply H.
+
+- destruct S; inversion Hs. unfold ptree_formula. unfold subst_ind_fit. fold subst_ind_fit. rewrite H1.
+  destruct H as [[[H2 H3] H4] H5].
+  assert (subst_ind_fit (ptree_formula P) (lor_ind S2 S1) = true) as Z. rewrite H2. simpl. apply and_bool_symm; auto.
+  pose proof (IHP H3 (lor_ind S2 S1) Z) as Ht. unfold neg_w_rule_sub_ptree_fit. fold neg_w_rule_sub_ptree_fit.
+  rewrite neg_w_rule_ptree_formula_true; auto.
+  assert ((neg_w_rule_term P E n H3 (lor_ind S2 S1) Z) = (neg_w_rule_term (exchange_ab f f0 n0 o P) E n (H2,H3,H4,H5) (lor_ind S1 S2) Hs)) as Z1. admit.
+  destruct Z1. repeat split; auto.
+  + rewrite neg_w_rule_ptree_formula.
+  + rewrite <- neg_w_rule_ptree_deg; auto.
+  + rewrite neg_w_rule_ptree_ord; auto.
+
+- simpl. destruct S; try destruct S1; inversion Hs.
+  rewrite H1. simpl. inversion H as [[[H4 H5] H6] H7].
+  destruct (and_bool_prop _ _ H1). clear H1.
+  destruct (and_bool_prop _ _ H0). clear H0.
+  repeat split; rewrite neg_w_rule_ptree_formula_true.
+  + admit.
+  + rewrite H4. simpl. rewrite H1, H2, H3. auto.
+  + admit.
+  + rewrite H4. simpl. rewrite H1, H2, H3. auto.
+  + rewrite <- neg_w_rule_ptree_deg; auto.
+  + rewrite H4. simpl. rewrite H1, H2, H3. auto.
+  + rewrite neg_w_rule_ptree_ord; auto.
+  + rewrite H4. simpl. rewrite H1, H2, H3. auto.
+
+- simpl. destruct S; try destruct S1; inversion Hs.
+  rewrite H1. simpl. inversion H as [[[H4 H5] H6] H7].
+  destruct (and_bool_prop _ _ H1). clear H1.
+  destruct (and_bool_prop _ _ H0). clear H0.
+  repeat split; rewrite neg_w_rule_ptree_formula_true.
+  + admit.
+  + rewrite H4. simpl. rewrite H1, H2, H3. auto.
+  + admit.
+  + rewrite H4. simpl. rewrite H1, H2, H3. auto.
+  + rewrite <- neg_w_rule_ptree_deg; auto.
+  + rewrite H4. simpl. rewrite H1, H2, H3. auto.
+  + rewrite neg_w_rule_ptree_ord; auto.
+  + rewrite H4. simpl. rewrite H1, H2, H3. auto.
+
+- simpl. destruct S; try destruct S1; try destruct S1_1; inversion Hs.
+  rewrite H1. simpl. inversion H as [[[H5 H6] H7] H8].
+  destruct (and_bool_prop _ _ H1). clear H1.
+  destruct (and_bool_prop _ _ H0). clear H0.
+  destruct (and_bool_prop _ _ H1). clear H1.
+  repeat split; rewrite neg_w_rule_ptree_formula_true.
+  + admit.
+  + rewrite H5. simpl. rewrite H0, H2, H3, H4. auto.
+  + admit.
+  + rewrite H5. simpl. rewrite H0, H2, H3, H4. auto.
+  + rewrite <- neg_w_rule_ptree_deg; auto.
+  + rewrite H5. simpl. rewrite H0, H2, H3, H4. auto.
+  + rewrite neg_w_rule_ptree_ord; auto.
+  + rewrite H5. simpl. rewrite H0, H2, H3, H4. auto.
+
+- simpl. inversion Hs. rewrite H1. inversion H as [[[H2 H3] H4] H5].
+  repeat split; rewrite neg_w_rule_ptree_formula_true.
+  + admit.
+  + rewrite H2. simpl. rewrite H1. auto.
+  + admit.
+  + rewrite H2. simpl. rewrite H1. auto.
+  + rewrite <- neg_w_rule_ptree_deg; auto.
+  + rewrite H2. simpl. rewrite H1. auto.
+  + rewrite neg_w_rule_ptree_ord; auto.
+  + rewrite H2. simpl. rewrite H1. auto.
+
+- simpl. destruct S; inversion Hs. rewrite H1.
+  inversion H as [[[H2 H3] H4] H5]. destruct (and_bool_prop _ _ H1).
+  repeat split; rewrite neg_w_rule_ptree_formula_true.
+  + admit.
+  + rewrite H2. simpl. rewrite H0, H6. auto.
+  + admit.
+  + rewrite H2. simpl. rewrite H0, H6. auto.
+  + rewrite <- neg_w_rule_ptree_deg; auto.
+  + rewrite H2. simpl. rewrite H0, H6. auto.
+  + rewrite neg_w_rule_ptree_ord; auto.
+  + rewrite H2. simpl. rewrite H0, H6. auto.
+
+- simpl. destruct S; inversion Hs. rewrite H1. simpl.
+  inversion H as [[[[H2 H3] H4] H5] H6]. destruct (and_bool_prop _ _ H1).
+  repeat split; try rewrite neg_w_rule_ptree_formula_true; try rewrite H2; auto.
+  + admit.
+  + apply neg_w_rule_sub_formula_closed. auto. apply neg_w_rule_counter_closed.
+  + admit.
+  + rewrite <- neg_w_rule_ptree_deg; auto.
+  + rewrite neg_w_rule_ptree_ord; auto.
+
+- simpl. destruct S; apply H.
+
+- simpl. destruct S; try apply H.
+  destruct H as [[[[[[[H2 H3] H4] H5] H6] H7] H8] H9].
+  assert (subst_ind_fit (ptree_formula P1) (lor_ind (0) S2) = true) as Z. inversion Hs. rewrite H2. destruct S1; simpl; auto. inversion H0.
+  assert (subst_ind_fit (ptree_formula P1) (lor_ind (1) S2) = true) as Z1. inversion Hs. rewrite H2. destruct S1; simpl; auto. inversion H0.
+  assert (subst_ind_fit (ptree_formula P2) (lor_ind (0) S2) = true) as Z2. inversion Hs. rewrite H4. destruct S1; simpl; auto. inversion H0.
+  assert (subst_ind_fit (ptree_formula P2) (lor_ind (1) S2) = true) as Z3. inversion Hs. rewrite H4. destruct S1; simpl; auto. inversion H0.
+  destruct S1; inversion Hs; rewrite H0; simpl.
+  + repeat split; rewrite neg_w_rule_ptree_formula_true; auto.
+    * admit.
+    * admit.
+    * admit.
+    * admit.
+    * rewrite H6. rewrite <- neg_w_rule_ptree_deg; auto.
+    * rewrite H7. rewrite <- neg_w_rule_ptree_deg; auto.
+    * rewrite neg_w_rule_ptree_ord; auto.
+    * rewrite neg_w_rule_ptree_ord; auto.
+  + repeat split; rewrite neg_w_rule_ptree_formula_true; auto.
+    * admit.
+    * admit.
+    * admit.
+    * admit.
+    * rewrite H6. rewrite <- neg_w_rule_ptree_deg; auto.
+    * rewrite H7. rewrite <- neg_w_rule_ptree_deg; auto.
+    * rewrite neg_w_rule_ptree_ord; auto.
+    * rewrite neg_w_rule_ptree_ord; auto.
+
+- simpl. destruct S; destruct (eq_f f E); apply H.
+
+- simpl. inversion H as [[[H1 H2] H3] H4]. destruct S; auto.
+  destruct S1; auto; destruct (subst_ind_fit f0 S2) eqn:HS2; simpl;
+  repeat split; auto; rewrite neg_w_rule_ptree_formula_true;
+  try apply IHP; auto; try rewrite H1; simpl; try rewrite non_target_fit,HS2;
+  try rewrite w_rule_ptree_deg; try rewrite w_rule_ptree_ord; auto.
+  + admit.
+  + admit.
+  + rewrite <- neg_w_rule_ptree_deg; auto.
+  + rewrite neg_w_rule_ptree_ord; auto.
+  + admit.
+  + admit.
+  + rewrite <- neg_w_rule_ptree_deg; auto.
+  + rewrite neg_w_rule_ptree_ord; auto.
+
+- simpl. inversion H as [[[[H0 H1] H2] H3] H4]. destruct S; auto; case (eq_f f E) eqn:X; case (eq_nat n0 n) eqn:X1; case (eq_term (neg_w_rule_counter (quantification_a f n0 t n1 o P) E n H (0)) t) eqn:X2; case (eq_term (neg_w_rule_counter (quantification_a f n0 t n1 o P) E n H (1)) t) eqn:X3; simpl; auto; repeat split; auto; rewrite H4; try apply ord_succ_monot; auto; apply ord_succ_nf; apply ptree_ord_nf; auto.
+
+- simpl. destruct S; try apply H. inversion H as [[[[H0 H1] H2] H3] H4].
+  assert (subst_ind_fit (ptree_formula P) (lor_ind (0) S2) = true). rewrite H0. simpl. destruct S1; inversion Hs; rewrite H6; auto.
+  assert (subst_ind_fit (ptree_formula P) (lor_ind (1) S2) = true). rewrite H0. simpl. destruct S1; inversion Hs; rewrite H7; auto.
+  destruct S1; inversion Hs; simpl; auto; rewrite neg_w_rule_ptree_formula_true; try rewrite H7; try rewrite H8; auto; simpl; repeat split; auto.
+  + case (eq_f f E).
+    * case (eq_nat n0 n).
+      --  case (eq_term (neg_w_rule_counter (quantification_ad f f0 n0 t n1 o P) E n H (lor_ind (0) S2)) t).
+          ++ repeat split; auto.
+             **  admit.
+             **  apply neg_w_rule_counter_closed.
+             **  admit.
+             **  rewrite <- neg_w_rule_ptree_deg; auto.
+             **  rewrite neg_w_rule_ptree_ord; auto.
+          ++  repeat split; auto.
+              **  admit.
+              **  apply neg_w_rule_counter_closed.
+              **  admit.
+              **  rewrite <- neg_w_rule_ptree_deg; auto.
+              **  rewrite neg_w_rule_ptree_ord; auto.
+      --  repeat split; auto.
+          ++  admit.
+          ++  apply neg_w_rule_counter_closed.
+          ++  admit.
+          ++  rewrite <- neg_w_rule_ptree_deg; auto.
+          ++  rewrite neg_w_rule_ptree_ord; auto.
+    * repeat split; auto.
+      --  admit.
+      --  apply neg_w_rule_counter_closed.
+      --  admit.
+      --  rewrite <- neg_w_rule_ptree_deg; auto.
+      --  rewrite neg_w_rule_ptree_ord; auto.
+    + case (eq_f f E).
+      * case (eq_nat n0 n).
+        --  case (eq_term (neg_w_rule_counter (quantification_ad f f0 n0 t n1 o P) E n H (lor_ind (1) S2)) t).
+            ++ repeat split; auto; rewrite H4. apply ord_succ_monot. apply ord_succ_nf. apply ptree_ord_nf; auto.
+            ++  repeat split; auto.
+                **  admit.
+                **  apply neg_w_rule_counter_closed.
+                **  admit.
+                **  rewrite <- neg_w_rule_ptree_deg; auto.
+                **  rewrite neg_w_rule_ptree_ord; auto.
+        --  repeat split; auto.
+            ++  admit.
+            ++  apply neg_w_rule_counter_closed.
+            ++  admit.
+            ++  rewrite <- neg_w_rule_ptree_deg; auto.
+            ++  rewrite neg_w_rule_ptree_ord; auto.
+      * repeat split; auto.
+        --  admit.
+        --  apply neg_w_rule_counter_closed.
+        --  admit.
+        --  rewrite <- neg_w_rule_ptree_deg; auto.
+        --  rewrite neg_w_rule_ptree_ord; auto.
+    
+
+- rewrite Hs. simpl. intros. destruct (H m) as [[[H1 H2] H3] H4]. fold valid in H2. repeat split; auto.
+
+- rewrite Hs. simpl. destruct S; inversion Hs. simpl; intros; destruct (H m) as [[[X1 X2] X3] X4]; fold valid in X2; assert (subst_ind_fit (ptree_formula (p m)) (lor_ind (non_target f) S2) = true). rewrite X1. simpl. destruct S1; inversion Hs; rewrite H2; rewrite (non_target_term_sub f n0 (represent m)); rewrite non_target_fit; auto. destruct S1; inversion Hs; simpl; auto; rewrite neg_w_rule_ptree_formula_true; auto; repeat split; auto.
+  + admit.
+  + admit.
+  + rewrite <- neg_w_rule_ptree_deg; auto.
+  + rewrite neg_w_rule_ptree_ord; auto.
+  + admit.
+  + admit.
+  + rewrite <- neg_w_rule_ptree_deg; auto.
+  + rewrite neg_w_rule_ptree_ord; auto. 
+
+- clear IHP2. rewrite Hs. inversion H as [[[[[[[H1 H2] H3] H4] H5] H6] H7] H8]. inversion Hs. assert (subst_ind_fit (ptree_formula P1) (lor_ind S (non_target f0)) = true). rewrite H1. simpl. rewrite H9. rewrite non_target_fit. auto.
+  repeat split; auto; rewrite neg_w_rule_ptree_formula_true; auto.
+  + admit.
+  + admit.
+  + rewrite <- neg_w_rule_ptree_deg; auto.
+  + rewrite neg_w_rule_ptree_ord; auto.
+
+- clear IHP1. rewrite Hs. inversion H as [[[[[[[H1 H2] H3] H4] H5] H6] H7] H8]. inversion Hs. assert (subst_ind_fit (ptree_formula P2) (lor_ind (0) S) = true). rewrite H3. simpl. rewrite H9. auto.
+  repeat split; auto; rewrite neg_w_rule_ptree_formula_true; auto.
+  + admit.
+  + admit.
+  + rewrite <- neg_w_rule_ptree_deg; auto.
+  + rewrite neg_w_rule_ptree_ord; auto.
+
+- rewrite Hs. inversion H as [[[[[[[H1 H2] H3] H4] H5] H6] H7] H8].
+  destruct S; try inversion Hs.
+  destruct (and_bool_prop _ _ H9) as [H10 H11].
+  assert (subst_ind_fit (ptree_formula P1) (lor_ind S1 (non_target f0)) = true). rewrite H1. simpl. rewrite H10. rewrite non_target_fit. auto.
+  assert (subst_ind_fit (ptree_formula P2) (lor_ind (0) S2) = true). rewrite H3. simpl. rewrite H11. auto.
+  simpl. repeat split; rewrite neg_w_rule_ptree_formula_true; auto.
+  + admit.
+  + admit.
+  + admit.
+  + admit.
+  + rewrite <- neg_w_rule_ptree_deg; auto.
+  + rewrite <- neg_w_rule_ptree_deg; auto.
+  + rewrite neg_w_rule_ptree_ord; auto.
+  + rewrite neg_w_rule_ptree_ord; auto.
+Admitted.
 
 
 
